books/projects/atomic-stobjs/constructors/frame$a.lisp
@@ -1,0 +1,749 @@
+;;; Copyright 2025 J. David Taylor
+;;;
+;;; Redistribution and use in source and binary forms, with or without
+;;; modification, are permitted provided that the following conditions are met:
+;;;
+;;; 1. Redistributions of source code must retain the above copyright notice,
+;;;    this list of conditions and the following disclaimer.
+;;;
+;;; 2. Redistributions in binary form must reproduce the above copyright notice,
+;;;    this list of conditions and the following disclaimer in the documentation
+;;;    and/or other materials provided with the distribution.
+;;;
+;;; 3. Neither the name of the copyright holder nor the names of its
+;;;    contributors may be used to endorse or promote products derived from this
+;;;    software without specific prior written permission.
+;;;
+;;; THIS SOFTWARE IS PROVIDED BY THE COPYRIGHT HOLDERS AND CONTRIBUTORS "AS IS"
+;;; AND ANY EXPRESS OR IMPLIED WARRANTIES, INCLUDING, BUT NOT LIMITED TO, THE
+;;; IMPLIED WARRANTIES OF MERCHANTABILITY AND FITNESS FOR A PARTICULAR PURPOSE
+;;; ARE DISCLAIMED. IN NO EVENT SHALL THE COPYRIGHT HOLDER OR CONTRIBUTORS BE
+;;; LIABLE FOR ANY DIRECT, INDIRECT, INCIDENTAL, SPECIAL, EXEMPLARY, OR
+;;; CONSEQUENTIAL DAMAGES (INCLUDING, BUT NOT LIMITED TO, PROCUREMENT OF
+;;; SUBSTITUTE GOODS OR SERVICES; LOSS OF USE, DATA, OR PROFITS; OR BUSINESS
+;;; INTERRUPTION) HOWEVER CAUSED AND ON ANY THEORY OF LIABILITY, WHETHER IN
+;;; CONTRACT, STRICT LIABILITY, OR TORT (INCLUDING NEGLIGENCE OR OTHERWISE)
+;;; ARISING IN ANY WAY OUT OF THE USE OF THIS SOFTWARE, EVEN IF ADVISED OF THE
+;;; POSSIBILITY OF SUCH DAMAGE.
+
+
+(in-package "ATOMIC-STOBJS")
+(set-verify-guards-eagerness 2)
+
+#||
+(include-book "std/lists/top" :dir :system)
+||#
+
+(include-book "../type-spec")
+(include-book "../utilities/top")
+
+
+;;;; Constants
+(defconst *field-keywords$a*
+  '(:recognizer :fixer :stobj :initial-element :accessor :updater))
+
+(defconst *body-keywords$a*
+  '(:recognizer :creator :fixer :view :debug))
+
+
+;;;; `DEFINE-FRAME$A' Predicates
+(defun frame$a-descriptor-p (descriptor)
+  (declare (xargs :guard t))
+  (and (consp descriptor)
+       (let ((name (car descriptor))
+             (kvl (cdr descriptor)))
+         (and (symbolp name)
+              (keyword-value-listp kvl)
+              (subsetp (evens kvl) *field-keywords$a* :test 'eq)
+              (let ((recognizer (cadr (assoc-keyword :recognizer kvl)))
+                    (fixer (cadr (assoc-keyword :fixer kvl)))
+                    (stobj (cadr (assoc-keyword :stobj kvl)))
+                    (initial-element (cadr (assoc-keyword :initial-element kvl)))
+                    (accessor (cadr (assoc-keyword :accessor kvl)))
+                    (updater (cadr (assoc-keyword :updater kvl))))
+                (declare (ignore initial-element))
+                (and (symbolp recognizer)
+                     (symbolp fixer)
+                     (or (and (not recognizer)
+                              (not fixer))
+                         (and recognizer
+                              fixer))
+                     (symbolp stobj)
+                     (symbolp accessor)
+                     (symbolp updater)))))))
+
+(defun frame$a-descriptor-list-p (fds)
+  (declare (xargs :guard t))
+  (if (atom fds)
+      (null fds)
+      (and (frame$a-descriptor-p (car fds))
+           (frame$a-descriptor-list-p (cdr fds)))))
+
+(defun frame$a-body-p (body)
+  (declare (xargs :guard t))
+  (and (true-listp body)
+       (if (consp (car body))
+           (and (frame$a-descriptor-p (car body))
+                (frame$a-body-p (cdr body)))
+           (and (keyword-value-listp body)
+                (subsetp (evens body) *body-keywords$a* :test 'eq)
+                (let ((recognizer (cadr (assoc-keyword :recognizer body)))
+                      (creator (cadr (assoc-keyword :creator body)))
+                      (fixer (cadr (assoc-keyword :fixer body)))
+                      (view (cadr (assoc-keyword :view body)))
+                      (debug (cadr (assoc-keyword :debug body))))
+                  (and (symbolp recognizer)
+                       (symbolp creator)
+                       (symbolp fixer)
+                       (symbolp view)
+                       (booleanp debug)))))))
+
+(defthm frame$a-body-p-when-frame$a-descriptor-list-p
+  (implies (frame$a-descriptor-list-p fds)
+           (frame$a-body-p fds))
+  :hints
+  (("Goal"
+    :induct (len fds))))
+
+(defun frame$a-form-p (form)
+  (declare (xargs :guard t))
+  (and (true-listp form)
+       (eq (car form) 'define-frame$a)
+       (symbolp (cadr form))
+       (frame$a-body-p (cddr form))))
+
+
+;;;; `DEFINE-FRAME$A' Parser
+(with-books (("std/lists/rev" :dir :system))
+  (defun split-body$a (fds body)
+    (declare (xargs :guard (and (frame$a-descriptor-list-p fds)
+                                (frame$a-body-p body))))
+    (if (or (atom body)
+            (atom (car body)))
+        (mv (reverse fds) body)
+        (split-body$a (cons (car body) fds) (cdr body))))
+
+  (local
+    (defthm frame$a-descriptor-list-p-of-rev
+      (implies (frame$a-descriptor-list-p fds)
+               (frame$a-descriptor-list-p (acl2::rev fds)))
+      :hints
+      (("Goal"
+        :in-theory (disable frame$a-descriptor-p)))))
+
+  (defthm split-body$a-values
+    (implies (and (frame$a-descriptor-list-p fds)
+                  (frame$a-body-p body))
+             (mv-let (fds kvl)
+                     (split-body$a fds body)
+               (and (frame$a-descriptor-list-p fds)
+                    (frame$a-body-p kvl)
+                    (keyword-value-listp kvl))))))
+
+(defun parse-fds$a (fds fields recognizers fixers stobjs
+                    initial-elements accessors updaters)
+  (declare (xargs :guard (and (frame$a-descriptor-list-p fds)
+                              (symbol-listp fields)
+                              (symbol-listp recognizers)
+                              (symbol-listp fixers)
+                              (symbol-listp stobjs)
+                              (true-listp initial-elements)
+                              (symbol-listp accessors)
+                              (symbol-listp updaters))))
+  (if (atom fds)
+      (mv (reverse fields)
+          (reverse recognizers)
+          (reverse fixers)
+          (reverse stobjs)
+          (reverse initial-elements)
+          (reverse accessors)
+          (reverse updaters))
+      (let* ((descriptor (car fds))
+             (field (car descriptor))
+             (kvl (cdr descriptor))
+             (recognizer (cadr (assoc-keyword :recognizer kvl)))
+             (fixer (cadr (assoc-keyword :fixer kvl)))
+             (stobj (cadr (assoc-keyword :stobj kvl)))
+             (initial-element (cadr (assoc-keyword :initial-element kvl)))
+             (accessor (cadr (assoc-keyword :accessor kvl)))
+             (updater (cadr (assoc-keyword :updater kvl))))
+        (parse-fds$a (cdr fds)
+                     (cons field fields)
+                     (cons recognizer recognizers)
+                     (cons fixer fixers)
+                     (cons stobj stobjs)
+                     (cons initial-element initial-elements)
+                     (cons accessor accessors)
+                     (cons updater updaters)))))
+
+(defun parse-kvl$a (kvl)
+  (declare (xargs :guard (and (frame$a-body-p kvl)
+                              (keyword-value-listp kvl))))
+  (let* ((recognizer (cadr (assoc-keyword :recognizer kvl)))
+         (creator (cadr (assoc-keyword :creator kvl)))
+         (fixer (cadr (assoc-keyword :fixer kvl)))
+         (view (cadr (assoc-keyword :view kvl)))
+         (debug (cadr (assoc-keyword :debug kvl))))
+    (mv recognizer creator fixer view debug)))
+
+(defun parse-form$a (form)
+  (declare (xargs :guard (frame$a-form-p form)))
+  (let ((body (cddr form)))
+    (mv-let (fds kvl)
+            (split-body$a () body)
+      (mv-let (fields recognizers fixers stobjs
+                      initial-elements accessors updaters)
+              (parse-fds$a fds () () () () () () ())
+        (mv-let (recognizer creator fixer view debug)
+                (parse-kvl$a kvl)
+          (mv fields recognizers fixers stobjs
+              initial-elements accessors updaters
+              recognizer creator fixer view debug))))))
+
+
+;;;; `DEFINE-FRAME$A'
+(defmacro define-frame$a (&whole form frame &body body)
+  (declare (xargs :guard (frame$a-form-p form))
+           (ignore body))
+  (mv-let (fields recognizers fixers stobjs
+                  initial-elements accessors updaters
+                  recognizer creator fixer view debug)
+          (parse-form$a form)
+    `(with-output
+       ,@(and (not debug)
+              '#!acl2(:off (warning! observation prove event history proof-tree)
+                           :summary-off (rules)
+                           :gag-mode t))
+
+       (make-event
+         (let* ((frame ',frame)
+                (%frame (symbolicate frame "%" frame))
+                (fields ',fields)
+                (%fields (loop$ :for field :in fields
+                               :collect (symbolicate field "%" field)))
+
+                (stobjs ',stobjs)
+                (world (w state))
+                (stobj-property-list (loop$ :for stobj :in stobjs
+                                           :collect (getprop stobj 'stobj nil 'current-acl2-world world)))
+                (absstobj-info-list (loop$ :for stobj :in stobjs
+                                          :collect (getprop stobj 'absstobj-info nil 'current-acl2-world world)))
+                (stobj$a-property-alist (table-alist 'stobj$a-property world))
+                (stobj$a-property-list (loop$ :for stobj :in stobjs
+                                             :collect (cdr (assoc stobj stobj$a-property-alist))))
+                (recognizers ',recognizers)
+                (recognizers (loop$ :for recognizer :in recognizers
+                                   :as stobj-property :in stobj-property-list
+                                   :as absstobj-info :in absstobj-info-list
+                                   :as stobj$a-property :in stobj$a-property-list
+                                   :collect (cond
+                                              (recognizer)
+                                              (stobj$a-property
+                                               (first (second stobj$a-property)))
+                                              (absstobj-info
+                                               (second (second absstobj-info)))
+                                              (stobj-property
+                                               (caadr stobj-property)))))
+                (creators (loop$ :for stobj-property :in stobj-property-list
+                                :as absstobj-info :in absstobj-info-list
+                                :as stobj$a-property :in stobj$a-property-list
+                                :collect (cond
+                                           (stobj$a-property
+                                            (second (second stobj$a-property)))
+                                           (absstobj-info
+                                            (second (third absstobj-info)))
+                                           (stobj-property
+                                            (cdadr stobj-property)))))
+                (fixer-alist (table-alist 'fixer world))
+                (fixers ',fixers)
+                (fixers (loop$ :for fixer :in fixers
+                              :as stobj :in stobjs
+                              :as stobj-property :in stobj-property-list
+                              :as absstobj-info :in absstobj-info-list
+                              :as stobj$a-property :in stobj$a-property-list
+                              :collect (cond
+                                         (fixer)
+                                         (stobj$a-property
+                                          (third (second stobj$a-property)))
+                                         (t
+                                          (cdr (assoc stobj fixer-alist))))))
+                (initial-element-names (loop$ :for field :in fields
+                                             :collect (symbolicate frame "*" frame "-" field "-INITIAL-ELEMENT*")))
+                (initial-elements (loop$ :for initial-element-name :in initial-element-names
+                                        :as creator :in creators
+                                        :collect (if creator
+                                                     `(,creator)
+                                                     initial-element-name)))
+
+                (recognizer ',recognizer)
+                (creator ',creator)
+                (fixer ',fixer)
+                (view ',view)
+                (accessors ',accessors)
+                (updaters ',updaters)
+
+                (recognizer (or recognizer
+                                (symbolicate frame frame (make-predicate-suffix frame))))
+                (creator (or creator
+                             (symbolicate frame "CREATE-" frame)))
+                (fixer (or fixer
+                           (symbolicate frame frame "-FIX")))
+                (view (or view
+                          (symbolicate frame frame "-VIEW")))
+                (accessors (loop$ :for field :in fields
+                                 :as accessor :in accessors
+                                 :collect (or accessor
+                                              (symbolicate frame frame "-" field))))
+                (updaters (loop$ :for field :in fields
+                                :as updater :in updaters
+                                :collect (or updater
+                                             (symbolicate frame frame "-" field "-SET"))))
+
+                (frame-begin (symbolicate frame frame "-BEGIN"))
+                (frame-end (symbolicate frame frame "-END"))
+                (defconst-forms (loop$ :for initial-element-name :in initial-element-names
+                                      :as initial-element :in ',initial-elements
+                                      :as stobj-property :in stobj-property-list
+                                      :when (not stobj-property)
+                                      :collect `(defconst ,initial-element-name ',initial-element)))
+                (prologue
+                 `((deflabel ,frame-begin)
+
+                   ,@defconst-forms))
+
+                (recognizer{type-prescription} (symbolicate frame recognizer "{TYPE-PRESCRIPTION}"))
+                (recognizer{compound-recognizer} (symbolicate frame recognizer "{COMPOUND-RECOGNIZER}"))
+                (recognizer-of-creator (symbolicate frame recognizer "-OF-" creator))
+                (recognizer-of-view (symbolicate frame recognizer "-OF-" view))
+
+                (creator{type-prescription} (symbolicate frame creator "{TYPE-PRESCRIPTION}"))
+
+                (fixer{rewrite} (symbolicate frame fixer "{REWRITE}"))
+                (fixer-when-recognizer (symbolicate frame fixer "-WHEN-" recognizer))
+                (fixer-when-not-recognizer (symbolicate frame fixer "-WHEN-NOT-" recognizer))
+
+                (view{type-prescription} (symbolicate frame view "{TYPE-PRESCRIPTION}"))
+                (view-collapse (symbolicate frame view "-COLLAPSE"))
+                (view{rewrite} (symbolicate frame view "{REWRITE}"))
+
+                (frame-equal (symbolicate frame frame "-EQUAL"))
+                (frame-equal{forward-chaining} (symbolicate frame frame-equal "{FORWARD-CHAINING}"))
+
+                (frame-theorems (symbolicate frame frame "-THEOREMS"))
+                (frame-definitions (symbolicate frame frame "-DEFINITIONS"))
+                (frame-aggressive (symbolicate frame frame "-AGGRESSIVE"))
+                (epilogue
+                 `((in-theory
+                     (enable ,fixer{rewrite}
+                             ,view{rewrite}
+                             ,@(loop$ :for updater :in updaters
+                                     :collect (symbolicate frame updater "{REWRITE}"))))
+
+                   (deflabel ,frame-end)
+
+                   (deftheory-static ,frame-theorems
+                     (set-difference-theories
+                      (set-difference-theories
+                       (current-theory ',frame-end)
+                       (current-theory ',frame-begin))
+                      (function-theory ',frame-end)))
+
+                   (deftheory-static ,frame-definitions
+                     (set-difference-theories
+                      (set-difference-theories
+                       (current-theory ',frame-end)
+                       (current-theory ',frame-begin))
+                      (theory ',frame-theorems)))
+
+                   (deftheory-static ,frame-aggressive
+                     ',(append
+                        (list view-collapse)
+                        (loop$ :for i :from 1 :to (len fields)
+                              :as recognizer :in recognizers
+                              :when recognizer
+                              :collect (symbolicate frame view "-WHEN-NOT-" recognizer "-" i))
+                        (loop$ :for accessor :in accessors
+                              :collect (symbolicate frame accessor "-WHEN-NOT-" recognizer))))
+
+                   (in-theory
+                     (union-theories (current-theory ',frame-begin)
+                                     (theory ',frame-theorems)))))
+
+                (body
+                 `(encapsulate ()
+
+                    ,@(loop$ :for i :from 1 :to (len fields)
+                            :as field :in fields
+                            :as recognizer :in recognizers
+                            :when recognizer
+                            :collect `(local
+                                        (defthm ,(symbolicate "ATOMIC-STOBJS" "BOOLEANP-OF-" recognizer "-" i)
+                                          (booleanp (,recognizer ,field))
+                                          :rule-classes
+                                          (:rewrite
+                                           :type-prescription))))
+
+                    ,@(loop$ :for i :from 1 :to (len fields)
+                            :as initial-element :in initial-elements
+                            :as initial-element-name :in initial-element-names
+                            :as recognizer :in recognizers
+                            :when recognizer
+                            :collect `(local
+                                        (defthm ,(symbolicate "ATOMIC-STOBJS" recognizer "-OF-" initial-element "-" i)
+                                          (,recognizer ,initial-element)
+                                          ,@(and (equal initial-element initial-element-name)
+                                                 `(:rule-classes nil)))))
+
+                    ,@(loop$ :for i :from 1 :to (len fields)
+                            :as field :in fields
+                            :as recognizer :in recognizers
+                            :as fixer :in fixers
+                            :when (and recognizer
+                                       fixer)
+                            :collect `(local
+                                        (defthm ,(symbolicate "ATOMIC-STOBJS" recognizer "-OF-" fixer "-" i)
+                                          (,recognizer (,fixer ,field)))))
+
+                    ,@(loop$ :for i :from 1 :to (len fields)
+                            :as field :in fields
+                            :as recognizer :in recognizers
+                            :as fixer :in fixers
+                            :when (and recognizer
+                                       fixer)
+                            :collect `(local
+                                        (defthm ,(symbolicate "ATOMIC-STOBJS" fixer "-WHEN-" recognizer "-" i)
+                                          (implies (,recognizer ,field)
+                                                   (equal (,fixer ,field)
+                                                          ,field)))))
+
+                    ,@(loop$ :for i :from 1 :to (len fields)
+                            :as field :in fields
+                            :as initial-element :in initial-elements
+                            :as recognizer :in recognizers
+                            :as fixer :in fixers
+                            :when (and recognizer
+                                       fixer)
+                            :collect `(local
+                                        (defthm ,(symbolicate "ATOMIC-STOBJS" fixer "-WHEN-NOT-" recognizer "-" i)
+                                          (implies (not (,recognizer ,field))
+                                                   (equal (,fixer ,field)
+                                                          ,initial-element)))))
+
+                    (local
+                      (in-theory
+                        (set-difference-theories
+                         (union-theories
+                          (union-theories (current-theory 'acl2::ground-zero)
+                                          (set-difference-theories
+                                           (universal-theory :here)
+                                           (universal-theory ',frame-begin)))
+                          '())
+                         '())))
+
+                    (defun ,recognizer (,frame)
+                      (declare (xargs :guard t))
+                      (and (true-listp ,frame)
+                           (= (len ,frame) ,(len fields))
+                           ,@(loop$ :for i :from 0 :to (1- (len fields))
+                                   :as recognizer :in recognizers
+                                   :when recognizer
+                                   :collect `(,recognizer (nth ,i ,frame)))
+                           t))
+
+                    (defun ,creator ()
+                      (declare (xargs :guard t))
+                      (list ,@initial-elements))
+
+                    (in-theory
+                      (disable (:e ,creator)))
+
+                    (defun ,fixer (,frame)
+                      (declare (xargs :guard (,recognizer ,frame)))
+                      (if (,recognizer ,frame)
+                          ,frame
+                          (,creator)))
+
+                    (defun ,view (,@fields ,frame)
+                      (declare (xargs :guard ,(if fields
+                                                  `(and ,@(loop$ :for field :in fields
+                                                                :as recognizer :in recognizers
+                                                                :when recognizer
+                                                                :collect `(,recognizer ,field))
+                                                        (,recognizer ,frame))
+                                                  `(,recognizer ,frame)))
+                               (ignore ,frame))
+                      (let (,@(loop$ :for field :in fields
+                                    :as fixer :in fixers
+                                    :when fixer
+                                    :collect `(,field (,fixer ,field))))
+                        (list ,@fields)))
+
+                    ,@(loop$ :for i :from 0 :to (1- (len fields))
+                            :as field-fixer :in fixers
+                            :as accessor :in accessors
+                            :collect `(defun ,accessor (,frame)
+                                        (declare (xargs :guard (,recognizer ,frame)))
+                                        (let ((,frame (,fixer ,frame)))
+                                          ,(if field-fixer
+                                               `(,field-fixer (nth ,i ,frame))
+                                               `(nth ,i ,frame)))))
+
+                    ,@(loop$ :for i :from 0 :to (1- (len fields))
+                            :as field :in fields
+                            :as field-recognizer :in recognizers
+                            :as field-fixer :in fixers
+                            :as updater :in updaters
+                            :collect `(defun ,updater (,field ,frame)
+                                        (declare (xargs :guard ,(if field-recognizer
+                                                                    `(and (,field-recognizer ,field)
+                                                                          (,recognizer ,frame))
+                                                                    `(,recognizer ,frame))))
+                                        (let (,@(and field-fixer
+                                                     `((,field (,field-fixer ,field))))
+                                              (,frame (,fixer ,frame)))
+                                          (update-nth ,i ,field ,frame))))
+
+                    ;; `RECOGNIZER'
+                    (defthm ,recognizer{type-prescription}
+                      (booleanp (,recognizer ,frame))
+                      :rule-classes :type-prescription)
+
+                    (defthm ,recognizer{compound-recognizer}
+                      (implies (,recognizer ,frame)
+                               ,(if (null fields)
+                                    `(null ,frame)
+                                    `(and (consp ,frame)
+                                          (true-listp ,frame))))
+                      :rule-classes :compound-recognizer)
+
+                    (defthm ,recognizer-of-creator
+                      (,recognizer (,creator)))
+
+                    (defthm ,recognizer-of-view
+                      (,recognizer (,view ,@fields ,frame)))
+
+                    ;; `CREATOR'
+                    (defthm ,creator{type-prescription}
+                      ,(if (null fields)
+                           `(null (,creator))
+                           `(and (consp (,creator))
+                                 (true-listp (,creator))))
+                      :rule-classes :type-prescription)
+
+                    ;; `FIXER'
+                    (with-books (("std/lists/nth" :dir :system))
+                      (local
+                        (defthm nth-of-cons
+                          (equal (nth i (cons a d))
+                                 (if (zp i)
+                                     a
+                                     (nth (1- i) d)))))
+
+                      (local
+                        (in-theory
+                          (disable nth
+                                   acl2::nth-when-zp)))
+
+                      (defthmd ,fixer{rewrite}
+                        (equal (,fixer ,frame)
+                               (,view ,@(loop$ :for accessor :in accessors
+                                              :collect `(,accessor ,frame))
+                                      ,frame))
+                        :hints
+                        ((acl2::equal-by-nths-hint))))
+
+                    (defthm ,fixer-when-recognizer
+                      (implies (,recognizer ,frame)
+                               (equal (,fixer ,frame)
+                                      ,frame)))
+
+                    (defthm ,fixer-when-not-recognizer
+                      (implies (not (,recognizer ,frame))
+                               (equal (,fixer ,frame)
+                                      (,creator))))
+
+                    ;; `VIEW'
+                    (defthm ,view{type-prescription}
+                      ,(if (null fields)
+                           `(null (,view ,frame))
+                           `(and (consp (,view ,@fields ,frame))
+                                 (true-listp (,view ,@fields ,frame))))
+                      :rule-classes :type-prescription)
+
+                    (with-books (("std/lists/nth" :dir :system))
+                      (local
+                        (defthm nth-of-cons
+                          (equal (nth i (cons a d))
+                                 (if (zp i)
+                                     a
+                                     (nth (1- i) d)))))
+
+                      (local
+                        (in-theory
+                          (disable nth
+                                   acl2::nth-when-zp)))
+
+                      (defthmd ,view-collapse
+                        (implies (case-split (,recognizer ,%frame))
+                                 (equal (,view ,@(loop$ :for accessor :in accessors
+                                                       :collect `(,accessor ,%frame))
+                                               ,frame)
+                                        ,%frame))
+                        :hints
+                        ((acl2::equal-by-nths-hint))))
+
+                    (defthmd ,view{rewrite}
+                      (implies (syntaxp (not (and (consp ,frame)
+                                                  (eq (car ,frame) ',creator))))
+                               (equal (,view ,@fields ,frame)
+                                      (,view ,@fields (,creator)))))
+
+                    ,@(loop$ :for i :from 1 :to (len fields)
+                            :as j :from 0 :to (1- (len fields))
+                            :as field :in fields
+                            :as recognizer :in recognizers
+                            :as initial-element :in initial-elements
+                            :when recognizer
+                            :collect `(defthmd ,(symbolicate frame view "-WHEN-NOT-" recognizer "-" i)
+                                        (implies (not (,recognizer ,field))
+                                                 (equal (,view ,@fields ,frame)
+                                                        (,view ,@(update-nth j initial-element fields) ,frame)))))
+
+                    ,@(loop$ :for i :from 1 :to (len fields)
+                            :as j :from 0 :to (1- (len fields))
+                            :as field :in fields
+                            :as fixer :in fixers
+                            :when fixer
+                            :collect `(defthm ,(symbolicate frame view "-OF-" fixer "-" i)
+                                        (equal (,view ,@(update-nth j `(,fixer ,field) fields) ,frame)
+                                               (,view ,@fields ,frame))))
+
+                    ;; `ACCESSORS'
+                    ,@(loop$ :for i :from 1 :to (len fields)
+                            :as recognizer :in recognizers
+                            :as accessor :in accessors
+                            :when recognizer
+                            :collect `(defthm ,(symbolicate frame recognizer "-OF-" accessor "-" i)
+                                        (,recognizer (,accessor ,frame))
+                                        :rule-classes
+                                        (:rewrite
+                                         :type-prescription)))
+
+                    ,@(loop$ :for accessor :in accessors
+                            :as initial-element :in initial-elements
+                            :collect `(defthmd ,(symbolicate frame accessor "-WHEN-NOT-" recognizer)
+                                        (implies (not (,recognizer ,frame))
+                                                 (equal (,accessor ,frame)
+                                                        ,initial-element))))
+
+                    ,@(loop$ :for accessor :in accessors
+                            :as initial-element :in initial-elements
+                            :collect `(defthm ,(symbolicate frame accessor "-OF-" creator)
+                                        (equal (,accessor (,creator))
+                                               ,initial-element)))
+
+                    ,@(loop$ :for field :in fields
+                            :as fixer :in fixers
+                            :as accessor :in accessors
+                            :collect `(defthm ,(symbolicate frame accessor "-OF-" view)
+                                        (equal (,accessor (,view ,@fields ,frame))
+                                               ,(if fixer
+                                                    `(,fixer ,field)
+                                                    field))))
+
+                    ;; `UPDATERS'
+                    ,@(and fields
+                           `((with-books (("std/lists/nth" :dir :system))
+                               (local
+                                 (defthm nth-of-cons
+                                   (equal (nth i (cons a d))
+                                          (if (zp i)
+                                              a
+                                              (nth (1- i) d)))))
+
+                               (local
+                                 (in-theory
+                                   (disable nth
+                                            acl2::nth-when-zp)))
+
+                               ,@(let ((arguments (loop$ :for accessor :in accessors
+                                                        :collect `(,accessor ,frame))))
+                                   (loop$ :for i :from 0 :to (1- (len fields))
+                                         :as field :in fields
+                                         :as updater :in updaters
+                                         :collect `(defthmd ,(symbolicate frame updater "{REWRITE}")
+                                                     (implies (syntaxp (not (and (consp ,frame)
+                                                                                 (eq (car ,frame) ',view))))
+                                                              (equal (,updater ,field ,frame)
+                                                                     (,view ,@(update-nth i field arguments) ,frame)))
+                                                     :hints
+                                                     ((acl2::equal-by-nths-hint))))))))
+
+                    ,@(loop$ :for i :from 0 :to (1- (len fields))
+                            :as %field :in %fields
+                            :as updater :in updaters
+                            :collect `(defthm ,(symbolicate frame updater "-OF-" view)
+                                        (equal (,updater ,%field (,view ,@fields ,frame))
+                                               (,view ,@(update-nth i %field fields) ,frame))))
+
+                    ;; `FRAME-EQUAL'
+                    (defun-nx ,frame-equal (,%frame ,frame)
+                      (declare (xargs :guard t
+                                      :verify-guards nil))
+                      (and (,recognizer ,%frame)
+                           (,recognizer ,frame)
+                           ,@(loop$ :for accessor :in accessors
+                                   :collect `(equal (,accessor ,%frame)
+                                                    (,accessor ,frame)))))
+
+                    (with-books (("std/lists/nth" :dir :system))
+                      (local
+                        (defthm nth-of-cons
+                          (equal (nth i (cons a d))
+                                 (if (zp i)
+                                     a
+                                     (nth (1- i) d)))))
+
+                      (local
+                        (in-theory
+                          (disable nth
+                                   acl2::nth-when-zp)))
+
+                      (defthm ,frame-equal{forward-chaining}
+                        (implies (,frame-equal ,%frame ,frame)
+                                 (equal ,%frame ,frame))
+                        :rule-classes
+                        ((:forward-chaining :trigger-terms
+                                            ((,frame-equal ,%frame ,frame))
+                                            :corollary
+                                            (implies t
+                                                     (implies (,frame-equal ,%frame ,frame)
+                                                              (equal ,%frame ,frame)))))
+                        :hints
+                        ((acl2::equal-by-nths-hint)
+                         ,@(and fields
+                                `(("Subgoal 1"
+                                   :cases ,(loop$ :for i :from 0 :to (1- (len fields))
+                                                 :collect `(equal acl2::n ,i))))))))))
+
+                (stobj$a-property `(stobj$a-property (,recognizer
+                                                      ,creator
+                                                      ,fixer
+                                                      ,frame-equal)
+                                                     (,fields
+                                                      ,recognizers
+                                                      ,initial-element-names
+                                                      ,fixers
+                                                      ,stobjs
+                                                      ,accessors
+                                                      ,updaters
+                                                      (,view)))))
+
+           `(progn
+              ,@prologue
+
+              ,body
+
+              ,@epilogue
+
+              (table stobj$a-property ',frame ',stobj$a-property)))))))
