books/projects/atomic-stobjs/.dir-locals.el
@@ -58,11 +58,21 @@
 
 ;;; Atomic-Stobjs
                (eval . (put 'with-books 'common-lisp-indent-function 1))
-               (eval . (put 'define-vector$c 'common-lisp-indent-function 2))
-               (eval . (put 'define-vector$a 'common-lisp-indent-function 2))
-               (eval . (put 'define-vector$corr 'common-lisp-indent-function 1))
-               (eval . (put 'define-vector$abs 'common-lisp-indent-function 1))
+               (eval . (put 'define-hash-table 'common-lisp-indent-function 2))
+               (eval . (put 'define-hash-table$a 'common-lisp-indent-function 2))
+               (eval . (put 'define-hash-table$abs 'common-lisp-indent-function 1))
+               (eval . (put 'define-hash-table$c 'common-lisp-indent-function 2))
+               (eval . (put 'define-hash-table$corr 'common-lisp-indent-function 1))
+               (eval . (put 'define-frame 'common-lisp-indent-function 1))
+               (eval . (put 'define-frame$a 'common-lisp-indent-function 1))
+               (eval . (put 'define-frame$abs 'common-lisp-indent-function 1))
+               (eval . (put 'define-frame$c 'common-lisp-indent-function 1))
+               (eval . (put 'define-frame$corr 'common-lisp-indent-function 1))
                (eval . (put 'define-vector 'common-lisp-indent-function 2))
+               (eval . (put 'define-vector$a 'common-lisp-indent-function 2))
+               (eval . (put 'define-vector$abs 'common-lisp-indent-function 1))
+               (eval . (put 'define-vector$c 'common-lisp-indent-function 2))
+               (eval . (put 'define-vector$corr 'common-lisp-indent-function 1))
 
                ))
  (shell-mode . (
